stlc finished.

exercises/Stlc.v
@@ -107,8 +107,300 @@ Inductive substi (s:tm) (x:id) : tm -> tm -> Prop :=
 
 Hint Constructors substi.
 
+Hint Resolve eq_id.
+Hint Resolve neq_id.
+Hint Unfold subst.
+
 Theorem substi_correct : forall s x t t',
   [x:=s]t = t' <-> substi s x t t'.
 Proof.
-  (* FILL IN HERE *) Admitted.
-(** [] *)
+  intros s x t t'. split.
+  Case "->"; generalize dependent t'; induction t; intros t' H; simpl in H; try(destruct (eq_id_dec x i));subst; auto.
+  Case "<-"; intros; induction H;subst; simpl; try(rewrite eq_id); try(rewrite neq_id); auto.
+Qed.
+
+(* Reduction *)
+
+Reserved Notation "t1 '==>' t2" (at level 40).
+
+Inductive step : tm -> tm -> Prop :=
+  | ST_AppAbs : forall x T t12 v2,
+         value v2 ->
+         (tapp (tabs x T t12) v2) ==> [x:=v2]t12
+  | ST_App1 : forall t1 t1' t2,
+         t1 ==> t1' ->
+         tapp t1 t2 ==> tapp t1' t2
+  | ST_App2 : forall v1 t2 t2',
+         value v1 ->
+         t2 ==> t2' ->
+         tapp v1 t2 ==> tapp v1  t2'
+  | ST_IfTrue : forall t1 t2,
+      (tif ttrue t1 t2) ==> t1
+  | ST_IfFalse : forall t1 t2,
+      (tif tfalse t1 t2) ==> t2
+  | ST_If : forall t1 t1' t2 t3,
+      t1 ==> t1' ->
+      (tif t1 t2 t3) ==> (tif t1' t2 t3)
+
+where "t1 '==>' t2" := (step t1 t2).
+
+Tactic Notation "step_cases" tactic(first) ident(c) :=
+  first;
+  [ Case_aux c "ST_AppAbs" | Case_aux c "ST_App1"
+  | Case_aux c "ST_App2" | Case_aux c "ST_IfTrue"
+  | Case_aux c "ST_IfFalse" | Case_aux c "ST_If" ].
+
+Hint Constructors step.
+
+Notation multistep := (multi step).
+Notation "t1 '==>*' t2" := (multistep t1 t2) (at level 40).
+
+(* example *)
+
+Lemma step_example1 :
+  (tapp idBB idB) ==>* idB.
+Proof.
+  eapply multi_step.
+    apply ST_AppAbs.
+    apply v_abs.
+  simpl.
+  apply multi_refl.  Qed.
+
+Lemma step_example2 :
+  (tapp idBB (tapp idBB idB)) ==>* idB.
+Proof.
+  eapply multi_step.
+    apply ST_App2. auto.
+    apply ST_AppAbs. auto.
+  eapply multi_step.
+    apply ST_AppAbs. simpl. auto.
+  simpl. apply multi_refl.  Qed.
+
+Lemma step_example3 :
+  tapp (tapp idBB notB) ttrue ==>* tfalse.
+Proof.
+  eapply multi_step.
+    apply ST_App1. apply ST_AppAbs. auto. simpl.
+  eapply multi_step.
+    apply ST_AppAbs. auto. simpl.
+  eapply multi_step.
+    apply ST_IfTrue. apply multi_refl.  Qed.
+
+Lemma step_example4 :
+  tapp idBB (tapp notB ttrue) ==>* tfalse.
+Proof.
+  eapply multi_step.
+    apply ST_App2. auto.
+    apply ST_AppAbs. auto. simpl.
+  eapply multi_step.
+    apply ST_App2. auto.
+    apply ST_IfTrue.
+  eapply multi_step.
+    apply ST_AppAbs. auto. simpl.
+  apply multi_refl.  Qed.
+
+Lemma step_example1' :
+  (tapp idBB idB) ==>* idB.
+Proof. normalize.  Qed.
+
+Lemma step_example2' :
+  (tapp idBB (tapp idBB idB)) ==>* idB.
+Proof.
+  normalize.
+Qed.
+
+Lemma step_example3' :
+  tapp (tapp idBB notB) ttrue ==>* tfalse.
+Proof. normalize.  Qed.
+
+Lemma step_example4' :
+  tapp idBB (tapp notB ttrue) ==>* tfalse.
+Proof. normalize.  Qed.
+
+(* Exercise: 2 stars (step_example3) *)
+
+Lemma step_example5 :
+       (tapp (tapp idBBBB idBB) idB)
+  ==>* idB.
+Proof.
+  normalize.
+Qed.
+
+Lemma step_example5' :
+       (tapp (tapp idBBBB idBB) idB)
+  ==>* idB.
+Proof.
+  eapply multi_step. eauto.
+  eapply multi_step. simpl. eauto.
+  simpl. eauto.
+Qed.
+
+(* Typing *)
+
+(* context *)
+
+Module PartialMap.
+
+Definition partial_map (A:Type) := id -> option A.
+
+Definition empty {A:Type} : partial_map A := (fun _ => None).
+
+Definition extend {A:Type} (Gamma : partial_map A) (x:id) (T : A) :=
+  fun x' => if eq_id_dec x x' then Some T else Gamma x'.
+
+Lemma extend_eq : forall A (ctxt: partial_map A) x T,
+  (extend ctxt x T) x = Some T.
+Proof.
+  intros. unfold extend. rewrite eq_id. auto.
+Qed.
+
+Lemma extend_neq : forall A (ctxt: partial_map A) x1 T x2,
+  x2 <> x1 ->
+  (extend ctxt x2 T) x1 = ctxt x1.
+Proof.
+  intros. unfold extend. rewrite neq_id; auto.
+Qed.
+
+End PartialMap.
+
+Definition context := partial_map ty.
+
+(* Typing Relation *)
+
+Reserved Notation "Gamma '|-' t '\in' T" (at level 40).
+
+Inductive has_type : context -> tm -> ty -> Prop :=
+  | T_Var : forall Gamma x T,
+      Gamma x = Some T ->
+      Gamma |- tvar x \in T
+  | T_Abs : forall Gamma x T11 T12 t12,
+      extend Gamma x T11 |- t12 \in T12 ->
+      Gamma |- tabs x T11 t12 \in TArrow T11 T12
+  | T_App : forall T11 T12 Gamma t1 t2,
+      Gamma |- t1 \in TArrow T11 T12 ->
+      Gamma |- t2 \in T11 ->
+      Gamma |- tapp t1 t2 \in T12
+  | T_True : forall Gamma,
+       Gamma |- ttrue \in TBool
+  | T_False : forall Gamma,
+       Gamma |- tfalse \in TBool
+  | T_If : forall t1 t2 t3 T Gamma,
+       Gamma |- t1 \in TBool ->
+       Gamma |- t2 \in T ->
+       Gamma |- t3 \in T ->
+       Gamma |- tif t1 t2 t3 \in T
+
+where "Gamma '|-' t '\in' T" := (has_type Gamma t T).
+
+Tactic Notation "has_type_cases" tactic(first) ident(c) :=
+  first;
+  [ Case_aux c "T_Var" | Case_aux c "T_Abs"
+  | Case_aux c "T_App" | Case_aux c "T_True"
+  | Case_aux c "T_False" | Case_aux c "T_If" ].
+
+Hint Constructors has_type.
+
+(* Examples *)
+
+Example typing_example_1 :
+  empty |- tabs x TBool (tvar x) \in TArrow TBool TBool.
+Proof.
+  apply T_Abs. apply T_Var. reflexivity.  Qed.
+
+Example typing_example_1' :
+  empty |- tabs x TBool (tvar x) \in TArrow TBool TBool.
+Proof. auto.  Qed.
+
+Example typing_example_2 :
+  empty |-
+    (tabs x TBool
+       (tabs y (TArrow TBool TBool)
+          (tapp (tvar y) (tapp (tvar y) (tvar x))))) \in
+    (TArrow TBool (TArrow (TArrow TBool TBool) TBool)).
+Proof with auto using extend_eq.
+  apply T_Abs.
+  apply T_Abs.
+  eapply T_App. apply T_Var...
+  eapply T_App. apply T_Var...
+  apply T_Var...
+Qed.
+
+(* Exercise: 2 stars, optional (typing_example_2_full) *)
+
+Example typing_example_2_full :
+  empty |-
+    (tabs x TBool
+       (tabs y (TArrow TBool TBool)
+          (tapp (tvar y) (tapp (tvar y) (tvar x))))) \in
+    (TArrow TBool (TArrow (TArrow TBool TBool) TBool)).
+Proof with auto.
+  apply T_Abs.
+  apply T_Abs.
+  eapply T_App. apply T_Var. eapply extend_eq.
+  eapply T_App. apply T_Var. eapply extend_eq.
+  eapply T_Var. eapply extend_neq. intros contra. solve by inversion.
+Qed.
+
+(* Exercise: 2 stars (typing_example_3) *)
+
+Lemma extend_find: forall A (ctxt: partial_map A) x2 x1 r T,
+  x2 <> x1 ->
+  ctxt x1 = r ->
+  (extend ctxt x2 T) x1 = r.
+Proof.
+  intros. subst. apply extend_neq. assumption.
+Qed.
+
+Example typing_example_3 :
+  exists T,
+    empty |-
+      (tabs x (TArrow TBool TBool)
+         (tabs y (TArrow TBool TBool)
+            (tabs z TBool
+               (tapp (tvar y) (tapp (tvar x) (tvar z)))))) \in
+      T.
+Proof with auto.
+  eapply ex_intro. repeat (apply T_Abs). eapply T_App.
+  apply T_Var. eapply extend_find. intros H. solve by inversion. apply extend_eq.
+  eapply T_App.
+  eapply T_Var. eapply extend_find. intros H. solve by inversion.
+  eapply extend_find. intros H. solve by inversion.
+  apply extend_eq.
+  eapply T_Var. apply extend_eq.
+Qed.
+
+Example typing_nonexample_1 :
+  ~ exists T,
+      empty |-
+        (tabs x TBool
+            (tabs y TBool
+               (tapp (tvar x) (tvar y)))) \in
+        T.
+Proof.
+  intros Hc. inversion Hc.
+  (* The [clear] tactic is useful here for tidying away bits of
+     the context that we're not going to need again. *)
+  inversion H. subst. clear H.
+  inversion H5. subst. clear H5.
+  inversion H4. subst. clear H4.
+  inversion H2. subst. clear H2.
+  inversion H5. subst. clear H5.
+  (* rewrite extend_neq in H1. rewrite extend_eq in H1. *)
+  inversion H1.  Qed.
+
+(* Exercise: 3 stars, optional (typing_nonexample_3) *)
+
+Example typing_nonexample_3 :
+  ~ (exists S, exists T,
+        empty |-
+          (tabs x S
+             (tapp (tvar x) (tvar x))) \in
+          T).
+Proof.
+  intros contra.
+  inv contra. inv H.
+  inv H0. inv H5. inv H2. inv H1. inv H4. inversion H1. clear H1. induction T11; induction T12; try(solve by inversion 3).
+  apply IHT11_1. inversion H0. rewrite <- H2 in *. rewrite H1. assumption.
+  apply IHT11_1. inversion H0. rewrite <- H2 in *. rewrite H1. assumption.
+Qed.
+End STLC.
